Core models fixes.

hax-lib/proof-libs/fstar/core/Alloc.Collections.Vec_deque.fsti
@@ -1,24 +1,29 @@
 module Alloc.Collections.Vec_deque
+#set-options "--fuel 0 --ifuel 1 --z3rlimit 15"
+open FStar.Mul
 open Rust_primitives
 
-type t_VecDeque: Type0 -> unit -> Type0
+type t_VecDeque (v_T: Type0) (v_A: Type0) =
+  | VecDeque : Rust_primitives.Seq.t_Seq v_T v_A -> t_VecDeque v_T v_A
 
-val impl_5__push_back #t #a (v: t_VecDeque t a) (x: t): t_VecDeque t a
+val impl_5__push_back (#v_T #v_A: Type0) (self: t_VecDeque v_T v_A) (x: v_T)
+    : Prims.Pure (t_VecDeque v_T v_A) Prims.l_True (fun _ -> Prims.l_True)
 
-val impl_5__len #t #a (v: t_VecDeque t a): usize
+val impl_5__len (#v_T #v_A: Type0) (self: t_VecDeque v_T v_A)
+    : Prims.Pure usize Prims.l_True (fun _ -> Prims.l_True)
 
-val impl_5__pop_front #t #a (v: t_VecDeque t a): t_VecDeque t a & Core_models.Option.t_Option t
+val impl_5__pop_front (#v_T #v_A: Type0) (self: t_VecDeque v_T v_A)
+    : Prims.Pure (t_VecDeque v_T v_A & Core_models.Option.t_Option v_T)
+      Prims.l_True
+      (fun _ -> Prims.l_True)
 
-
-[@FStar.Tactics.Typeclasses.tcinstance]
-val from_vec_deque_array t a n: Core_models.Convert.t_From (Alloc.Collections.Vec_deque.t_VecDeque t a)
-        (Rust_primitives.Arrays.t_Array t
-            (Rust_primitives.Integers.mk_usize n))
-
-[@FStar.Tactics.Typeclasses.tcinstance]
-val index_vec_deque t a: Core_models.Ops.Index.t_Index (Alloc.Collections.Vec_deque.t_VecDeque t a)
-        Rust_primitives.Integers.usize
-
-[@FStar.Tactics.Typeclasses.tcinstance]
-val update_at t a: Rust_primitives.Hax.update_at_tc (Alloc.Collections.Vec_deque.t_VecDeque t a)
-        Rust_primitives.Integers.usize
+[@@ FStar.Tactics.Typeclasses.tcinstance]
+let impl_6 (#v_T #v_A: Type0) : Core_models.Ops.Index.t_Index (t_VecDeque v_T v_A) usize =
+  {
+    f_Output = v_T;
+    f_index_pre = (fun (self: t_VecDeque v_T v_A) (i: usize) -> true);
+    f_index_post = (fun (self: t_VecDeque v_T v_A) (i: usize) (out: v_T) -> true);
+    f_index
+    =
+    fun (self: t_VecDeque v_T v_A) (i: usize) -> Rust_primitives.Seq.seq_index #v_T #v_A self._0 i
+  }
