hax-lib/proof-libs/fstar/core/Alloc.String.fst
@@ -1,21 +1,45 @@
 module Alloc.String
+#set-options "--fuel 0 --ifuel 1 --z3rlimit 15"
+open FStar.Mul
+open Rust_primitives
 
-type t_String = string
+type t_String = | String : string -> t_String
 
-let impl__String__new (): t_String = ""
+let impl_String__new (_: Prims.unit) : t_String = String "" <: t_String
 
-let impl__String__push_str (self: t_String) (s: t_String): t_String =
-    self ^ s
+let impl_String__push_str (self: t_String) (other: string) : t_String =
+  let self:t_String = String (Rust_primitives.String.str_concat self._0 other) <: t_String in
+  self
 
-let impl__String__push (self: t_String) (ch: FStar.Char.char) = 
-    self ^ (FStar.String.string_of_char ch)
+let impl_String__push (self: t_String) (c: char) : t_String =
+  let self:t_String =
+    String
+    (Rust_primitives.String.str_concat self._0 (Rust_primitives.String.str_of_char c <: string))
+    <:
+    t_String
+  in
+  self
 
-let impl__String__pop (self: t_String): (Alloc.String.t_String & Core_models.Option.t_Option FStar.Char.char) = 
-    let l = FStar.String.length self in 
-    if l > 0 then 
-        (FStar.String.sub self 0 (l - 1), Core_models.Option.Option_Some (FStar.String.index self (l - 1)))
-    else (self, Core_models.Option.Option_None)
-
-/// Placeholder for the to_string typeclass
-assume
-val f_to_string (#t: Type) {| Core_models.TypeClassPlaceHolder.t_Placeholder |} (x:t) : Alloc.String.t_String
+let impl_String__pop (self: t_String) : (t_String & Core_models.Option.t_Option char) =
+  let l:usize = Core_models.Str.impl_str__len self._0 in
+  let self, hax_temp_output:(t_String & Core_models.Option.t_Option char) =
+    if l >. mk_usize 0
+    then
+      let self:t_String =
+        String (Rust_primitives.String.str_sub self._0 (mk_usize 0) (l -! mk_usize 1 <: usize))
+        <:
+        t_String
+      in
+      self,
+      (Core_models.Option.Option_Some
+        (Rust_primitives.String.str_index self._0 (l -! mk_usize 1 <: usize))
+        <:
+        Core_models.Option.t_Option char)
+      <:
+      (t_String & Core_models.Option.t_Option char)
+    else
+      self, (Core_models.Option.Option_None <: Core_models.Option.t_Option char)
+      <:
+      (t_String & Core_models.Option.t_Option char)
+  in
+  self, hax_temp_output <: (t_String & Core_models.Option.t_Option char)
