hax-lib/proof-libs/fstar/core/Alloc.Collections.Binary_heap.fsti
@@ -1,27 +1,17 @@
 module Alloc.Collections.Binary_heap
+#set-options "--fuel 0 --ifuel 1 --z3rlimit 15"
+open FStar.Mul
 open Rust_primitives
 
-val t_BinaryHeap: Type -> unit -> eqtype
+val t_BinaryHeap (v_T v_U: Type0) : eqtype
 
-val impl_10__new: #t:Type -> (#[(Tactics.exact (`()))]_:unit) -> t_BinaryHeap t ()
-val impl_10__push: #t:Type -> (#[(Tactics.exact (`()))]_:unit) -> t_BinaryHeap t () -> t -> t_BinaryHeap t ()
-val impl_11__len: #t:Type -> (#[(Tactics.exact (`()))]_:unit) -> t_BinaryHeap t () -> usize
-val impl_11__iter: #t:Type -> (#[(Tactics.exact (`()))]_:unit) -> t_BinaryHeap t () -> t_Slice t
+val impl_9__new: #v_T: Type0 -> #v_U: Type0 -> Prims.unit
+  -> Prims.Pure (t_BinaryHeap v_T v_U) Prims.l_True (fun _ -> Prims.l_True)
 
-open Core_models.Option
+val impl_9__push (#v_T #v_U: Type0) (self: t_BinaryHeap v_T v_U) (v: v_T)
+    : Prims.Pure (t_BinaryHeap v_T v_U) Prims.l_True (fun _ -> Prims.l_True)
 
-val impl_11__peek: #t:Type -> (#[(Tactics.exact (`()))]_:unit) -> t_BinaryHeap t () -> t_Option t
-val impl_10__pop: #t:Type -> (#[(Tactics.exact (`()))]_:unit) -> t_BinaryHeap t () -> t_BinaryHeap t () & t_Option t
-
-unfold
-let nonempty h = v (impl_11__len h) > 0
-
-val lemma_peek_len: #t:Type -> (#[(Tactics.exact (`()))]_:unit) -> h: t_BinaryHeap t ()
-  -> Lemma (Option_Some? (impl_11__peek h) <==> nonempty h)
-  
-val lemma_pop_len: #t:Type -> (#[(Tactics.exact (`()))]_:unit) -> h: t_BinaryHeap t ()
-  -> Lemma (Option_Some? (snd (impl_10__pop h)) <==> nonempty h)
-
-val lemma_peek_pop: #t:Type -> (#[(Tactics.exact (`()))]_u:unit) -> h: t_BinaryHeap t ()
-  -> Lemma (impl_11__peek h == snd (impl_10__pop h))
-          [SMTPat (impl_11__peek #t #_u h)]
+val impl_9__pop (#v_T #v_U: Type0) (self: t_BinaryHeap v_T v_U)
+    : Prims.Pure (t_BinaryHeap v_T v_U & Core_models.Option.t_Option v_T)
+      Prims.l_True
+      (fun _ -> Prims.l_True)
