hax-lib/proof-libs/fstar/core/Std.Collections.Hash.Map.fsti
@@ -1,9 +1,19 @@
 module Std.Collections.Hash.Map
+#set-options "--fuel 0 --ifuel 1 --z3rlimit 15"
+open FStar.Mul
+open Rust_primitives
 
-val t_HashMap (k v s:Type0): eqtype
+val t_HashMap (v_K v_V v_S: Type0) : eqtype
 
-val impl__new #k #v: unit -> t_HashMap k v Std.Hash.Random.t_RandomState
+val impl__new: #v_K: Type0 -> #v_V: Type0 -> Prims.unit
+  -> Prims.Pure (t_HashMap v_K v_V Std.Hash.Random.t_RandomState)
+      Prims.l_True
+      (fun _ -> Prims.l_True)
 
-val impl_2__get #k #v #s (#y:Type0): t_HashMap k v s -> k -> Core_models.Option.t_Option v
+val impl_2__get (#v_K #v_V #v_S #v_Y: Type0) (m: t_HashMap v_K v_V v_S) (k: v_K)
+    : Prims.Pure (Core_models.Option.t_Option v_V) Prims.l_True (fun _ -> Prims.l_True)
 
-val impl_2__insert #k #v #s: t_HashMap k v s -> k -> v -> (t_HashMap k v s & Core_models.Option.t_Option v)
+val impl_2__insert (#v_K #v_V #v_S: Type0) (m: t_HashMap v_K v_V v_S) (k: v_K) (v: v_V)
+    : Prims.Pure (t_HashMap v_K v_V v_S & Core_models.Option.t_Option v_V)
+      Prims.l_True
+      (fun _ -> Prims.l_True)
